ArkLib.lean
@@ -241,5 +241,6 @@ import ArkLib.ToVCVio.EvalDist.Instances.OptionT
 import ArkLib.ToVCVio.OracleComp.Coercions.SubSpec
 import ArkLib.ToVCVio.OracleComp.EvalDist
 import ArkLib.ToVCVio.OracleComp.SimSemantics.SimulateQ
+import ArkLib.ToVCVio.Tactic.VCVNorm
 import ArkLib.ToVCVio.ToMathlib.Control.StateT
 import ArkLib.ToVCVio.ToMathlib.Data.Vector.Basic
